strengthen read_log_entry

steel/formats/everparse/Veritas.Formats.Pure.fst
@@ -3,3 +3,6 @@ module LP = LowParse.Spec.Base
 
 let serialize_length x =
   Veritas.Formats.EverParse.Value.value_size32 x
+
+let parsed s v =
+  LP.parse Veritas.Formats.EverParse.Vlog_entry.vlog_entry_parser s == Some (v, Seq.length s)
