steel/Veritas.Formats.fsti
@@ -7,18 +7,29 @@ module A = Steel.Array
 
 open Steel.Effect.Common
 open Steel.Effect
+open Steel.Reference
 
 val serialize_value: v:value -> dst: A.array U8.t { A.length dst == U32.v (serialize_length v) } ->
   SteelT unit
     (A.varray dst)
     (fun _ -> A.varray dst)
 
-val extract_log_entry_from (len: U32.t) (buf: A.array U8.t { A.length buf == U32.v len }) (pos: A.array (x: U32.t { U32.v x <= U32.v len }) { A.length pos == 1 })
-  : SteelT (option vlog_entry)
-    (A.varray buf `star` A.varray pos)
-    (fun _ -> A.varray buf `star` A.varray pos)
- (* /\
-            log at position h0.pos contains a vali repr of v *)
+val extract_log_entry_from (len: U32.t) (buf: A.array U8.t { A.length buf == U32.v len }) (pos: ref (x: U32.t { U32.v x <= U32.v len }))
+  : Steel (option vlog_entry)
+    (A.varray buf `star` vptr pos)
+    (fun _ -> A.varray buf `star` vptr pos)
+    (fun _ -> True)
+    (fun h res h' ->
+      let p = h (vptr pos) in
+      let p' = h' (vptr pos) in
+      U32.v p <= U32.v p' /\
+      h' (A.varray buf) == h (A.varray buf) /\
+      begin match res with
+      | None -> True
+      | Some v ->
+        parsed (Seq.slice (h (A.varray buf)) (U32.v p) (U32.v p')) v
+      end
+    )
 
 val serialize_stamped_record
   (dst: A.array U8.t { 184 <= A.length dst })
