steel/formats/Veritas.Formats.Pure.fsti
@@ -3,5 +3,8 @@ include Veritas.Formats.Aux
 include Veritas.Formats.Types
 
 module U32 = FStar.UInt32
+module U8 = FStar.UInt8
 
 val serialize_length : value -> (l: U32.t { U32.v l > 0 })
+
+val parsed: Seq.seq U8.t -> vlog_entry -> prop
